\documentclass{article}
\usepackage[utf8]{inputenc}
\usepackage{amsmath, amssymb}

\title{DSBA Calculus HW4}
\author{Kirill Korolev, 203-1}
\date{2th of October, 2020}

\begin{document}

\maketitle

\begin{enumerate}

\item Find the following limits:

\begin{enumerate}
\item $\lim_{n \to \infty} (\sqrt{n^2 + 1} - \sqrt{n^2 - 1}) \cdot \sin{(n^2 + 3)}$


Because $-1 \leq sin(n^2 + 3) \leq 1$
\begin{align*}
&x_n = -(\sqrt{n^2 + 1} - \sqrt{n^2 - 1}) \leq (\sqrt{n^2 + 1} - \sqrt{n^2 - 1}) \cdot \sin{(n^2 + 3)} \leq (\sqrt{n^2 + 1} - \sqrt{n^2 - 1}) = z_n\\
&\lim_{n \to \infty} x_n = \lim_{n \to \infty} -(\sqrt{n^2 + 1} - \sqrt{n^2 - 1}) = -\lim_{n \to \infty} \frac{2}{\sqrt{n^2 + 1} + \sqrt{n^2 - 1}} = 0\\
&\lim_{n \to \infty} z_n = \lim_{n \to \infty} (\sqrt{n^2 + 1} - \sqrt{n^2 - 1}) = \lim_{n \to \infty} \frac{2}{\sqrt{n^2 + 1} + \sqrt{n^2 - 1}} = 0\\
\end{align*}

Then by sandwich theorem:
\[\lim_{n \to \infty} (\sqrt{n^2 + 1} - \sqrt{n^2 - 1}) \cdot \sin{(n^2 + 3)}=0\]

\item $\lim_{n \to \infty} \frac{(4\cos{n} - 3n)^2(2n^5 - n^3 + 1)}{(6n^3 + 5n\sin{n})(n + 2)}$

\end{enumerate}

\end{enumerate}

\end{document}